ExistentialRules/Terms/ListsOfTerms.lean
@@ -1,57 +1,5 @@
+import BasicLeanDatastructures.List.AllListsOfLength
 import ExistentialRules.Terms.Basic
-
--- TODO: maybe extract this to basic data structures as this is generic for lists
-def all_lists_of_length (candidates : List α) : Nat -> List (List α)
-| .zero => [[]]
-| .succ n =>
-  let prev_terms := all_lists_of_length candidates n
-  candidates.flatMap (fun t =>
-    prev_terms.map (fun ts =>
-      t :: ts
-    )
-  )
-
--- TODO: same as above
-theorem mem_all_lists_of_length (candidates : List α) (length : Nat) : ∀ as, as ∈ (all_lists_of_length candidates length) ↔ (as.length = length ∧ (∀ a, a ∈ as -> a ∈ candidates)) := by
-  induction length with
-  | zero => intro as; unfold all_lists_of_length; simp; intro eq a mem; rw [eq] at mem; simp at mem
-  | succ length ih =>
-    intro as
-    unfold all_lists_of_length
-    simp only [List.mem_flatMap, List.mem_map]
-
-    constructor
-    . intro h
-      rcases h with ⟨a, a_mem, prev, prev_mem, as_eq⟩
-      rw [← as_eq]
-      specialize ih prev
-      have ih := ih.mp prev_mem
-      constructor
-      . rw [List.length_cons, ih.left]
-      . intro a' a'_mem
-        rw [List.mem_cons] at a'_mem
-        cases a'_mem with
-        | inl a'_mem => rw [a'_mem]; apply a_mem
-        | inr a'_mem => apply ih.right; exact a'_mem
-    . intro h
-      cases as with
-      | nil => simp at h
-      | cons hd tl =>
-        exists hd
-        constructor
-        . apply h.right
-          simp
-        . exists tl
-          constructor
-          . rw [ih]
-            constructor
-            . have l := h.left
-              rw [List.length_cons, Nat.add_right_cancel_iff] at l
-              exact l
-            . intro a a_mem
-              apply h.right
-              simp [a_mem]
-          . rfl
 
 variable {sig : Signature} [DecidableEq sig.C] [DecidableEq sig.V]
 
